Instructions.v
@@ -1,6 +1,8 @@
 Require Import Coqlib.
 Require Import MachineInt.
 
+(** Définitions des instructions. *)
+
 Inductive Instr : Set := 
   (* LOAD *)
   | LDA_ir : byte -> Instr
@@ -14,11 +16,32 @@ Inductive Instr : Set :=
   | STX_rm : nat -> Instr
   | STY_rm : nat -> Instr
   (* ARITHMETIC *)
+  | ADC_ir : byte -> Instr
+  | SBC_ir : byte -> Instr
   | ADC_mr : nat -> Instr
   | SBC_mr : nat -> Instr
+  (* BRANCHING *)
+  | BVC_i_rel : nat -> Instr
+  | BVS_i_rel : nat -> Instr
+  | BCC_i_rel : nat -> Instr
+  | BCS_i_rel : nat -> Instr
+  | BNE_i_rel : nat -> Instr
+  | BEQ_i_rel : nat -> Instr
+  | JMP_abs : word -> Instr
+  | JMP_ind : nat -> Instr
+  (* COMPARISION *)
+  | CMP_i : byte -> Instr
+  | CPX_i : byte -> Instr
+  | CPY_i : byte -> Instr
+  (* INCREMENT/DECREMENT *)
+  | INC : Instr
+  | INX : Instr
+  | INY : Instr
+  | DEC : Instr
+  | DEX : Instr
+  | DEY : Instr
   (* MISC *)
-  | NOP : Instr
-.
+  | NOP : Instr.
 
 Module Instructions.
 
