Main.v
@@ -1,20 +1,12 @@
-Require Import MachineInt.
-Require Import Coqlib.
-Require Import Repeat.
+(** Ce fichier contient une série de programmes dont le but est de vérifier 
+le bon fonctionnement de l'émulateur. *)
 
-Require Import Instructions.
+Require Import Coqlib.
+Require Import MachineInt.
+
 Require Import AbstractRegister.
 Require Import AbstractMachine.
-
-Definition StartR := AbstractRegister.mkState (Byte.repr 0) (Byte.repr 0) (Byte.repr 0).
-
-Definition StartM := repeat (Byte.repr 0) 4096.
-
-Definition StartPC := Word.repr 0.
-
-Definition StartST := AbstractMachine.mkState false false false false false false false.
-
-Definition StartP := (StartR, StartM, StartPC, StartST).
+Require Import Instructions.
 
 Definition prog1 : list Instr :=
   (LDA_ir (Byte.repr 1)) ::
@@ -26,7 +18,7 @@ Definition prog1 : list Instr :=
   (STX_rm 6) ::
   nil.
 
-Eval compute in run StartP prog1 100.
+Eval compute in run StartP prog1 (length prog1).
 
 Definition prog2 : list Instr :=
   (LDX_ir (Byte.repr 4)) ::
@@ -34,12 +26,44 @@ Definition prog2 : list Instr :=
   (LDX_mr 6) ::
   nil.
 
-Eval compute in run StartP prog2 2.
+Eval compute in run StartP prog2 (length prog2).
 
-Definition prog3 : list Instr :=
+Definition prog2bis : list Instr :=
   (LDX_ir (Byte.repr 4)) ::
   (LDX_mr 6) ::
   (STX_rm 6) ::
   nil.
 
-Eval compute in run StartP prog3 3.
+Eval compute in run StartP prog2bis (length prog2bis).
+
+Definition prog3 : list Instr :=
+  (LDX_ir (Byte.repr 1)) ::
+  (STX_rm 0) ::
+  (LDX_ir (Byte.repr 2)) ::
+  (STX_rm 1) ::
+  (LDX_ir (Byte.repr 3)) ::
+  (STX_rm 2) ::
+  (ADC_mr 0) ::
+  (ADC_mr 1) ::
+  (ADC_mr 2) ::
+  nil.
+
+Eval compute in run StartP prog3 (length prog3).
+
+Definition prog4 : list Instr :=
+  (LDX_ir (Byte.repr 1)) ::
+  (STX_rm 0) ::
+  (LDX_ir (Byte.repr 2)) ::
+  (STX_rm 1) ::
+  (LDX_ir (Byte.repr 3)) ::
+  (STX_rm 2) ::
+  (ADC_mr 0) ::
+  (ADC_mr 1) ::
+  (ADC_mr 2) ::
+  (SBC_mr 0) ::
+  (SBC_mr 1) ::
+  (SBC_mr 2) ::
+  (SBC_mr 2) ::
+  nil.
+
+Eval compute in run StartP prog4 (length prog4).
