Repeat.v
@@ -1,6 +1,8 @@
 Require Import MachineInt.
 Require Import List.
 
+(** Pris chez Coq 8.5. *)
+
 Section Repeat.
 
   Variable A : byte.
