README.md
@@ -1,0 +1,4 @@
+Launch `./refresh_makefile` after adding other files to the project.
+Launch `make` to compile all files in the project's folder.
+Launch `make html` to generate the documentation.
+Launch `make clean` to clean up all generated files.
